src/HOL/Library/Char_ord.thy
@@ -11,27 +11,29 @@ begin
 instantiation char :: linorder
 begin
 
-definition "c1 \<le> c2 \<longleftrightarrow> nat_of_char c1 \<le> nat_of_char c2"
-definition "c1 < c2 \<longleftrightarrow> nat_of_char c1 < nat_of_char c2"
+definition less_eq_char :: "char \<Rightarrow> char \<Rightarrow> bool"
+  where "c1 \<le> c2 \<longleftrightarrow> of_char c1 \<le> (of_char c2 :: nat)"
+
+definition less_char :: "char \<Rightarrow> char \<Rightarrow> bool"
+  where "c1 < c2 \<longleftrightarrow> of_char c1 < (of_char c2 :: nat)"
+
 
 instance
   by standard (auto simp add: less_eq_char_def less_char_def)
 
 end
 
-lemma less_eq_char_simps:
-  "0 \<le> c"
-  "Char k \<le> 0 \<longleftrightarrow> numeral k mod 256 = (0 :: nat)"
-  "Char k \<le> Char l \<longleftrightarrow> numeral k mod 256 \<le> (numeral l mod 256 :: nat)"
-  for c :: char
-  by (simp_all add: Char_def less_eq_char_def)
+lemma less_eq_char_simp [simp]:
+  "Char b0 b1 b2 b3 b4 b5 b6 b7 \<le> Char c0 c1 c2 c3 c4 c5 c6 c7
+    \<longleftrightarrow> foldr (\<lambda>b k. of_bool b + k * 2) [b0, b1, b2, b3, b4, b5, b6, b7] 0
+      \<le> foldr (\<lambda>b k. of_bool b + k * 2) [c0, c1, c2, c3, c4, c5, c6, c7] (0::nat)"
+  by (simp add: less_eq_char_def)
 
-lemma less_char_simps:
-  "\<not> c < 0"
-  "0 < Char k \<longleftrightarrow> (0 :: nat) < numeral k mod 256"
-  "Char k < Char l \<longleftrightarrow> numeral k mod 256 < (numeral l mod 256 :: nat)"
-  for c :: char
-  by (simp_all add: Char_def less_char_def)
+lemma less_char_simp [simp]:
+  "Char b0 b1 b2 b3 b4 b5 b6 b7 < Char c0 c1 c2 c3 c4 c5 c6 c7
+    \<longleftrightarrow> foldr (\<lambda>b k. of_bool b + k * 2) [b0, b1, b2, b3, b4, b5, b6, b7] 0
+      < foldr (\<lambda>b k. of_bool b + k * 2) [c0, c1, c2, c3, c4, c5, c6, c7] (0::nat)"
+  by (simp add: less_char_def)
 
 instantiation char :: distrib_lattice
 begin
@@ -43,40 +45,5 @@ instance
   by standard (auto simp add: inf_char_def sup_char_def max_min_distrib2)
 
 end
-
-instantiation String.literal :: linorder
-begin
-
-context includes literal.lifting
-begin
-
-lift_definition less_literal :: "String.literal \<Rightarrow> String.literal \<Rightarrow> bool"
-  is "ord.lexordp (<)" .
-
-lift_definition less_eq_literal :: "String.literal \<Rightarrow> String.literal \<Rightarrow> bool"
-  is "ord.lexordp_eq (<)" .
-
-instance
-proof -
-  interpret linorder "ord.lexordp_eq (<)" "ord.lexordp (<) :: string \<Rightarrow> string \<Rightarrow> bool"
-    by (rule linorder.lexordp_linorder[where less_eq="(\<le>)"]) unfold_locales
-  show "PROP ?thesis"
-    by intro_classes (transfer, simp add: less_le_not_le linear)+
-qed
-
-end
-
-end
-
-lemma less_literal_code [code]:
-  "(<) = (\<lambda>xs ys. ord.lexordp (<) (String.explode xs) (String.explode ys))"
-  by (simp add: less_literal.rep_eq fun_eq_iff)
-
-lemma less_eq_literal_code [code]:
-  "(\<le>) = (\<lambda>xs ys. ord.lexordp_eq (<) (String.explode xs) (String.explode ys))"
-  by (simp add: less_eq_literal.rep_eq fun_eq_iff)
-
-lifting_update literal.lifting
-lifting_forget literal.lifting
 
 end
